Move WeakeningEnv (and extends lemmas) before typing; remove BDEnvTyping completely

pcuic/theories/Conversion/PCUICWeakeningEnvConv.v
@@ -1,8 +1,8 @@
 (* Distributed under the terms of the MIT license. *)
 From MetaCoq.Template Require Import config utils.
 From MetaCoq.PCUIC Require Import PCUICAst PCUICAstUtils
-  PCUICEquality (* PCUICContextSubst *) (* PCUICUnivSubst *) (* PCUICCases *)
-  PCUICReduction PCUICCumulativity (* PCUICTyping *)
+  PCUICWeakeningEnv PCUICEquality PCUICReduction PCUICCumulativity PCUICCumulativitySpec
+  (* PCUICContextSubst *) (* PCUICUnivSubst *) (* PCUICCases *) (* PCUICTyping *)
   (* PCUICGuardCondition *) (* PCUICGlobalEnv *).
 From Equations Require Import Equations.
 
@@ -11,220 +11,47 @@ Require Import ssreflect.
 Set Default Goal Selector "!".
 Implicit Types (cf : checker_flags).
 
-Lemma global_ext_constraints_app Σ Σ' φ
-  : ConstraintSet.Subset (universes Σ).2 (universes Σ').2 ->
-    ConstraintSet.Subset (global_ext_constraints (Σ, φ))
-                         (global_ext_constraints (Σ', φ)).
+Lemma compare_term_subset {cf} pb Σ φ φ' t t'
+  : ConstraintSet.Subset φ φ'
+    -> compare_term pb Σ φ t t' -> compare_term pb Σ φ' t t'.
 Proof.
-  unfold global_ext_constraints; simpl.
-  intros sub ctr Hc. apply ConstraintSet.union_spec in Hc.
-  apply ConstraintSet.union_spec.
-  destruct Hc as [Hc|Hc]; [now left|right]. clear φ.
-  unfold global_constraints in Hc.
-  apply (sub _ Hc).
+  intro H. apply eq_term_upto_univ_impl; auto.
+  all: change eq_universe with (compare_universe Conv).
+  all: change leq_universe with (compare_universe Cumul).
+  3: destruct pb.
+  4: transitivity (compare_universe Cumul φ).
+  4: tc.
+  all: intros ??; now eapply cmp_universe_subset.
 Qed.
 
-Lemma satisfies_subset φ φ' val :
-  ConstraintSet.Subset φ φ' ->
-  satisfies val φ' ->
-  satisfies val φ.
-Proof.
-  intros sub sat ? isin.
-  apply sat, sub; auto.
-Qed.
-
-Lemma leq_universe_subset {cf:checker_flags} ctrs ctrs' t u
-  : ConstraintSet.Subset ctrs ctrs'
-    -> leq_universe ctrs t u -> leq_universe ctrs' t u.
-Proof.
-  intros Hctrs.
-  destruct t, u; cbnr; trivial.
-  intros H; unfold_univ_rel.
-  apply H.
-  eapply satisfies_subset; eauto.
-Qed.
-
-Lemma eq_universe_subset {cf:checker_flags} ctrs ctrs' t u
-  : ConstraintSet.Subset ctrs ctrs'
-    -> eq_universe ctrs t u -> eq_universe ctrs' t u.
-Proof.
-  intros Hctrs.
-  destruct t, u; cbnr; trivial.
-  intros H; unfold_univ_rel.
-  apply H.
-  eapply satisfies_subset; eauto.
-Qed.
+Lemma eq_term_subset {cf} Σ φ φ' t t'
+  : ConstraintSet.Subset φ φ' -> eq_term Σ φ t t' -> eq_term Σ φ' t t'.
+Proof. apply compare_term_subset with (pb := Conv). Qed.
 
 Lemma leq_term_subset {cf:checker_flags} Σ ctrs ctrs' t u
   : ConstraintSet.Subset ctrs ctrs' -> leq_term Σ ctrs t u -> leq_term Σ ctrs' t u.
+Proof. apply compare_term_subset with (pb := Cumul). Qed.
+
+Lemma compare_decl_subset {cf} pb Σ φ φ' d d'
+  : ConstraintSet.Subset φ φ'
+    -> compare_decl pb Σ φ d d' -> compare_decl pb Σ φ' d d'.
 Proof.
-  intro H. apply eq_term_upto_univ_impl; auto.
-  - intros t' u'. eapply eq_universe_subset; assumption.
-  - intros t' u'. eapply leq_universe_subset; assumption.
-  - intros t' u' eq. apply eq_universe_leq_universe'.
-    eapply eq_universe_subset; eauto.
+  intros Hφ []; constructor; eauto using compare_term_subset.
 Qed.
 
-(** * Weakening lemmas w.r.t. the global environment *)
+Lemma compare_context_subset {cf} pb Σ φ φ' Γ Γ'
+  : ConstraintSet.Subset φ φ'
+    -> compare_context pb Σ φ Γ Γ' ->  compare_context pb Σ φ' Γ Γ'.
+Proof.
+  intros Hφ. induction 1; constructor; auto; eapply compare_decl_subset; eassumption.
+Qed.
 
-Generalizable Variables Σ Γ t T.
-
-Section Extends.
+Section ExtendsWf.
   Context {cf : checker_flags}.
   Context {Pcmp: global_env_ext -> context -> conv_pb -> term -> term -> Type}.
   Context {P: global_env_ext -> context -> term -> typ_or_sort -> Type}.
 
   Let wf := on_global_env Pcmp P.
-
-Definition weaken_env_prop_full
-  (P : global_env_ext -> context -> term -> term -> Type) :=
-  forall (Σ : global_env_ext) (Σ' : global_env), 
-    wf Σ -> wf Σ' -> extends Σ.1 Σ' ->
-    forall Γ t T, P Σ Γ t T -> P (Σ', Σ.2) Γ t T.
-
-Lemma weakening_env_global_ext_levels Σ Σ' φ (H : extends Σ Σ') l
-  : LevelSet.In l (global_ext_levels (Σ, φ))
-    -> LevelSet.In l (global_ext_levels (Σ', φ)).
-Proof.
-  unfold global_ext_levels; simpl.
-  intros Hl. apply LevelSet.union_spec in Hl.
-  apply LevelSet.union_spec.
-  destruct Hl as [Hl|Hl]; [now left|right]. clear φ.
-  destruct H as [[lsub csub] [Σ'' eq]]; subst.
-  apply LevelSet.union_spec in Hl.
-  apply LevelSet.union_spec; intuition auto.
-Qed.
-
-Lemma weakening_env_global_ext_levels' Σ Σ' φ (H : extends Σ Σ') l
-  : LevelSet.mem l (global_ext_levels (Σ, φ))
-    -> LevelSet.mem l (global_ext_levels (Σ', φ)).
-Proof.
-  intro HH. apply LevelSet.mem_spec in HH.
-  now eapply LevelSet.mem_spec, weakening_env_global_ext_levels.
-Qed.
-
-Lemma weakening_env_global_ext_constraints Σ Σ' φ (H : extends Σ Σ')
-  : ConstraintSet.Subset (global_ext_constraints (Σ, φ))
-                         (global_ext_constraints (Σ', φ)).
-Proof.
-  destruct H as [sub [Σ'' eq]]. subst.
-  apply global_ext_constraints_app, sub.
-Qed.
-
-Lemma eq_term_subset Σ φ φ' t t'
-  : ConstraintSet.Subset φ φ'
-    -> eq_term Σ φ t t' -> eq_term Σ φ' t t'.
-Proof.
-  intro H. apply eq_term_upto_univ_impl; auto.
-  all: intros u u'; eapply eq_universe_subset; assumption.
-Qed.
-
-Lemma compare_term_subset le Σ φ φ' t t'
-  : ConstraintSet.Subset φ φ'
-    -> compare_term le Σ φ t t' -> compare_term le Σ φ' t t'.
-Proof.
-  destruct le; [apply eq_term_subset|apply leq_term_subset].
-Qed.
-
-Lemma compare_decl_subset le Σ φ φ' d d'
-  : ConstraintSet.Subset φ φ'
-    -> compare_decl le Σ φ d d' -> compare_decl le Σ φ' d d'.
-Proof.
-  intros Hφ []; constructor; eauto using compare_term_subset.
-Qed.
-
-Lemma compare_context_subset le Σ φ φ' Γ Γ'
-  : ConstraintSet.Subset φ φ'
-    -> compare_context le Σ φ Γ Γ' ->  compare_context le Σ φ' Γ Γ'.
-Proof.
-  intros Hφ. induction 1; constructor; auto; eapply compare_decl_subset; eassumption.
-Qed.
-
-Lemma lookup_global_Some_fresh Σ c decl :
-  lookup_global Σ c = Some decl -> ~ (fresh_global c Σ).
-Proof.
-  induction Σ; cbn. 1: congruence.
-  destruct (eqb_spec c a.1); subst.
-  - intros [= <-] H2. inv H2.
-    contradiction.
-  - intros H1 H2. apply IHΣ; tas.
-    now inv H2.
-Qed.
-
-Lemma lookup_env_Some_fresh Σ c decl :
-  lookup_env Σ c = Some decl -> ~ (fresh_global c Σ.(declarations)).
-Proof.
-  apply lookup_global_Some_fresh.
-Qed.
-
-Lemma extends_lookup Σ Σ' c decl :
-  wf Σ' ->
-  extends Σ Σ' ->
-  lookup_env Σ c = Some decl ->
-  lookup_env Σ' c = Some decl.
-Proof.
-  destruct Σ as [univs Σ], Σ' as [univs' Σ']; cbn.
-  intros [hu hΣ].
-  rewrite /lookup_env; intros [sub [Σ'' eq]]; cbn in *. subst Σ'.
-  induction Σ'' in hΣ, c, decl |- *.
-  - simpl. auto.
-  - intros hl. depelim hΣ. specialize (IHΣ'' c decl hΣ hl).
-    simpl in *.
-    destruct (eqb_spec c kn); subst; auto.
-    apply lookup_global_Some_fresh in IHΣ''; contradiction.
-Qed.
-Hint Resolve extends_lookup : extends.
-
-Lemma weakening_env_declared_constant :
-  forall (Σ : global_env) cst (decl : constant_body),
-    declared_constant Σ cst decl ->
-    forall Σ' : global_env, wf Σ' -> extends Σ Σ' -> declared_constant Σ' cst decl.
-Proof.
-  intros Σ cst decl H0 Σ' X2 H2.
-  eapply extends_lookup; eauto.
-Qed.
-Hint Resolve weakening_env_declared_constant : extends.
-
-Lemma weakening_env_declared_minductive `{CF:checker_flags}:
-  forall (Σ : global_env) ind decl,
-    declared_minductive Σ ind decl ->
-    forall Σ' : global_env, wf Σ' -> extends Σ Σ' -> declared_minductive Σ' ind decl.
-Proof.
-  intros Σ cst decl H0 Σ' X2 H2.
-  eapply extends_lookup; eauto.
-Qed.
-Hint Resolve weakening_env_declared_minductive : extends.
-
-Lemma weakening_env_declared_inductive:
-  forall (H : checker_flags) (Σ : global_env) ind mdecl decl,
-    declared_inductive Σ mdecl ind decl ->
-    forall Σ' : global_env, wf Σ' -> extends Σ Σ' -> declared_inductive Σ' mdecl ind decl.
-Proof.
-  intros H Σ cst decl H0 [Hmdecl Hidecl] Σ' X2 H2. split; eauto with extends.
-Qed.
-Hint Resolve weakening_env_declared_inductive : extends.
-
-Lemma weakening_env_declared_constructor :
-  forall (H : checker_flags) (Σ : global_env) ind mdecl idecl decl,
-    declared_constructor Σ idecl ind mdecl decl ->
-    forall Σ' : global_env, wf Σ' -> extends Σ Σ' ->
-    declared_constructor Σ' idecl ind mdecl decl.
-Proof.
-  intros H Σ cst mdecl idecl cdecl [Hidecl Hcdecl] Σ' X2 H2.
-  split; eauto with extends.
-Qed.
-Hint Resolve weakening_env_declared_constructor : extends.
-
-Lemma weakening_env_declared_projection :
-  forall (H : checker_flags) (Σ : global_env) ind mdecl idecl cdecl pdecl,
-    declared_projection Σ idecl ind mdecl cdecl pdecl ->
-    forall Σ' : global_env, wf Σ' -> extends Σ Σ' ->
-    declared_projection Σ' idecl ind mdecl cdecl pdecl.
-Proof.
-  intros H Σ cst mdecl idecl cdecl pdecl [Hidecl Hcdecl] Σ' X2 H2.
-  split; eauto with extends.
-Qed.
-Hint Resolve weakening_env_declared_projection : extends.
 
 Lemma global_variance_sigma_mon {Σ Σ' gr napp v} :
   wf Σ' -> extends Σ Σ' ->
@@ -308,35 +135,20 @@ Proof.
     try solve [econstructor; eauto with extends; solve_all].
 Qed.
 
-#[global] Instance subrel_extends_eq (Σ Σ' : global_env) (ϕ : universes_decl) : 
+Lemma weakening_env_cumul_gen pb Σ Σ' φ Γ M N :
+  wf Σ' ->
   extends Σ Σ' ->
-  RelationClasses.subrelation (eq_universe (global_ext_constraints (Σ, ϕ))) 
-    (eq_universe (global_ext_constraints (Σ', ϕ))).
+  cumulAlgo_gen (Σ, φ)  Γ pb M N ->
+  cumulAlgo_gen (Σ', φ) Γ pb M N.
 Proof.
-  intros ext u u'.
-  apply eq_universe_subset.
-  apply global_ext_constraints_app, ext.
-Qed.
-
-#[global] Instance subrel_extends_le (Σ Σ' : global_env) (ϕ : universes_decl) : 
-  extends Σ Σ' ->
-  RelationClasses.subrelation (leq_universe (global_ext_constraints (Σ, ϕ))) 
-    (leq_universe (global_ext_constraints (Σ', ϕ))).
-Proof.
-  intros ext u u'.
-  apply leq_universe_subset.
-  apply global_ext_constraints_app, ext.
-Qed.
-
-#[global] Instance subrel_extends_eq_le (Σ Σ' : global_env) (ϕ : universes_decl) : 
-  extends Σ Σ' ->
-  RelationClasses.subrelation (eq_universe (global_ext_constraints (Σ, ϕ))) 
-    (leq_universe (global_ext_constraints (Σ', ϕ))).
-Proof.
-  intros ext u u'. intros eq.
-  eapply eq_universe_leq_universe.
-  eapply eq_universe_subset; tea.
-  apply global_ext_constraints_app, ext.
+  intros wfΣ ext.
+  induction 1; simpl.
+  - econstructor. eapply compare_term_subset.
+    + now eapply global_ext_constraints_app.
+    + simpl in *. eapply eq_term_upto_univ_weaken_env in c; simpl; eauto.
+      all:typeclasses eauto.
+  - econstructor 2; eauto. eapply weakening_env_red1; eauto.
+  - econstructor 3; eauto. eapply weakening_env_red1; eauto.
 Qed.
 
 Lemma weakening_env_conv Σ Σ' φ Γ M N :
@@ -344,250 +156,105 @@ Lemma weakening_env_conv Σ Σ' φ Γ M N :
   extends Σ Σ' ->
   convAlgo (Σ, φ) Γ M N ->
   convAlgo (Σ', φ) Γ M N.
-Proof.
-  intros wfΣ ext.
-  induction 1; simpl.
-  - econstructor. eapply eq_term_subset.
-    + now eapply global_ext_constraints_app.
-    + simpl in *. eapply eq_term_upto_univ_weaken_env in c; simpl; eauto.
-      all:typeclasses eauto.
-  - econstructor 2; eauto. eapply weakening_env_red1; eauto.
-  - econstructor 3; eauto. eapply weakening_env_red1; eauto.
-Qed.
+Proof. apply weakening_env_cumul_gen with (pb := Conv). Qed.
 
 Lemma weakening_env_cumul Σ Σ' φ Γ M N :
   wf Σ' ->
   extends Σ Σ' ->
   cumulAlgo (Σ, φ) Γ M N ->
   cumulAlgo (Σ', φ) Γ M N.
-Proof.
-  intros wfΣ ext.
-  induction 1; simpl.
-  - econstructor. eapply leq_term_subset.
-    + now eapply global_ext_constraints_app.
-    + simpl in *. eapply eq_term_upto_univ_weaken_env in c; simpl; eauto.
-      all:typeclasses eauto.
-  - econstructor 2; eauto. eapply weakening_env_red1; eauto.
-  - econstructor 3; eauto. eapply weakening_env_red1; eauto.
-Qed.
+Proof. apply weakening_env_cumul_gen with (pb := Cumul). Qed.
 
-Lemma weakening_env_is_allowed_elimination Σ Σ' φ u allowed :
+
+Lemma weakening_env_cumulSpec0 Σ Σ' φ Γ pb M N :
+  wf Σ' ->
+  extends Σ Σ' ->
+  cumulSpec0 (Σ, φ) Γ pb M N ->
+  cumulSpec0 (Σ', φ) Γ pb M N.
+Proof.
+  intros HΣ' Hextends Ind.
+  pose proof (subrelations_leq_extends _ _  φ Hextends). revert H.
+  assert (RelationClasses.subrelation 
+          (eq_universe (global_ext_constraints (Σ,φ)))
+          (leq_universe (global_ext_constraints (Σ',φ)))). 
+  { typeclasses eauto. } revert H.
+  generalize (leq_universe (global_ext_constraints (Σ',φ))); intros Rle Hlee Hle . 
+  revert pb Γ M N Ind Σ' Rle Hle Hlee HΣ' Hextends. 
+  apply: (cumulSpec0_ind_all (Σ,φ)).
+  all:intros; try solve [econstructor; eauto with extends; intuition auto]. 
+  - eapply cumul_Evar. solve_all.
+  - eapply cumul_Case.
+    * destruct X as (Hparams & Hinst & Hctx & Hret & IHret). repeat split; tas.
+      + solve_all.
+      + eapply R_universe_instance_impl'; eauto; apply subrelations_extends; eauto.
+      + eapply IHret; eauto.
+    * solve_all.
+    * solve_all.
+  - eapply cumul_Fix; solve_all.
+  - eapply cumul_CoFix; solve_all.
+  - eapply cumul_Ind; eauto. 2:solve_all.
+    eapply @R_global_instance_weaken_env. 1,2,6:eauto. all: tc.
+  - eapply cumul_Construct; eauto. 2:solve_all.
+    eapply @R_global_instance_weaken_env. 1,2,6:eauto. all: tc.
+  - eapply cumul_Sort. eapply subrelations_compare_extends; tea.
+  - eapply cumul_Const. eapply R_universe_instance_impl'; eauto; tc.
+Defined.
+
+
+Lemma weakening_env_convSpec Σ Σ' φ Γ M N :
+  wf Σ' ->
+  extends Σ Σ' ->
+  convSpec (Σ, φ) Γ M N ->
+  convSpec (Σ', φ) Γ M N.
+Proof. apply weakening_env_cumulSpec0 with (pb := Conv). Qed.
+
+Lemma weakening_env_cumulSpec Σ Σ' φ Γ M N :
+  wf Σ' ->
+  extends Σ Σ' ->
+  cumulSpec (Σ, φ) Γ M N ->
+  cumulSpec (Σ', φ) Γ M N.
+Proof. apply weakening_env_cumulSpec0 with (pb := Cumul). Qed.
+
+Lemma weakening_env_conv_decls {Σ φ Σ' Γ Γ'} :
   wf Σ' -> extends Σ Σ' ->
-  is_allowed_elimination (global_ext_constraints (Σ, φ)) allowed u ->
-  is_allowed_elimination (global_ext_constraints (Σ', φ)) allowed u.
+  CRelationClasses.subrelation (conv_decls cumulSpec0 (Σ, φ) Γ Γ') (conv_decls cumulSpec0 (Σ', φ) Γ Γ').
 Proof.
-  destruct allowed; cbnr; trivial.
-  intros wfΣ ext [ | al]; auto.
-  destruct u; cbn in *; try elim al.
-  right.
-  unfold_univ_rel.
-  apply al.
-  eapply satisfies_subset; eauto.
-  apply global_ext_constraints_app, ext.
-Qed.
-Hint Resolve weakening_env_is_allowed_elimination : extends.
-
-Hint Resolve weakening_env_global_ext_levels : extends.
-
-Lemma weakening_env_consistent_instance Σ Σ' φ ctrs u (H : extends Σ Σ')
-  : consistent_instance_ext (Σ, φ) ctrs u
-    -> consistent_instance_ext (Σ', φ) ctrs u.
-Proof.
-    unfold consistent_instance_ext, consistent_instance.
-    intros X.
-    destruct ctrs; tas.
-    destruct X as (H0 & H1 & H2); repeat split; tas.
-    - eapply forallb_Forall in H0; eapply forallb_Forall, Forall_impl; tea.
-      intros x ?; now eapply weakening_env_global_ext_levels'.
-    - eapply valid_subset; tea;
-      now eapply weakening_env_global_ext_constraints.
-Qed.
-Hint Resolve weakening_env_consistent_instance : extends.
-
-Lemma global_levels_Set Σ :
-  LevelSet.In Level.lzero (global_levels Σ).
-Proof.
-  unfold global_levels. lsets.
+  intros wfΣ' ext d d' Hd; depelim Hd; constructor; tas;
+    eapply weakening_env_convSpec; tea.
 Qed.
 
-Lemma global_levels_set Σ :
-  LevelSet.Equal (LevelSet.union (LevelSet.singleton Level.lzero) (global_levels Σ))
-  (global_levels Σ).
+Lemma weakening_env_cumul_decls {Σ φ Σ' Γ Γ'} :
+  wf Σ' -> extends Σ Σ' ->
+  CRelationClasses.subrelation (cumul_decls cumulSpec0 (Σ, φ) Γ Γ') (cumul_decls cumulSpec0 (Σ', φ) Γ Γ').
 Proof.
-  apply LevelSetProp.union_subset_equal.
-  intros x hin. eapply LevelSet.singleton_spec in hin; subst x.
-  apply global_levels_Set.
+  intros wfΣ' ext d d' Hd; depelim Hd; constructor; tas;
+    (eapply weakening_env_convSpec || eapply weakening_env_cumulSpec); tea.
 Qed.
 
-Lemma global_levels_sub {univs univs'} : univs ⊂_cs univs' ->
-  LevelSet.Subset (global_levels univs) (global_levels univs').
+Lemma weakening_env_conv_ctx {Σ Σ' φ Γ Δ} :
+  wf Σ' ->
+  extends Σ Σ' ->
+  conv_context cumulSpec0 (Σ, φ) Γ Δ ->
+  conv_context cumulSpec0 (Σ', φ) Γ Δ.
 Proof.
-  unfold global_levels => sub.
-  intros x hin % LevelSet.union_spec. 
-  apply LevelSet.union_spec. 
-  intuition auto. left. now apply sub.
+  intros wfΣ' ext.
+  intros; eapply All2_fold_impl; tea => Γ0 Γ' d d'.
+  now eapply weakening_env_conv_decls.
 Qed.
 
-Lemma extends_wf_universe {Σ : global_env_ext} Σ' u : extends Σ Σ' -> wf Σ' ->
-  wf_universe Σ u -> wf_universe (Σ', Σ.2) u.
+
+Lemma weakening_env_cumul_ctx {Σ Σ' φ Γ Δ} :
+  wf Σ' ->
+  extends Σ Σ' ->
+  cumul_context cumulSpec0 (Σ, φ) Γ Δ ->
+  cumul_context cumulSpec0 (Σ', φ) Γ Δ.
 Proof.
-  destruct Σ as [Σ univ]; cbn.
-  intros [sub [Σ'' eq]] wfΣ'.
-  destruct u; simpl; auto.
-  intros Hl.
-  intros l inl; specialize (Hl l inl).
-  cbn.
-  unfold global_ext_levels.
-  eapply LevelSet.union_spec; simpl.
-  apply LevelSet.union_spec in Hl as [Hl|Hl]; cbn in Hl.
-  - simpl. simpl in Hl. now left.
-  - right. eapply global_levels_sub; tea.
+  intros wfΣ' ext.
+  intros; eapply All2_fold_impl; tea => Γ0 Γ' d d'.
+  now eapply weakening_env_cumul_decls.
 Qed.
 
-(* Lemma wf_extends {Σ Σ'} : wf Σ' -> extends Σ Σ' -> wf Σ.
-Proof.
-  intros HΣ' [univs [Σ'' eq]]. simpl in *.
-  split => //.
-  - red.
-  induction Σ''; auto.
-  inv HΣ'. auto.
-Qed. *)
+End ExtendsWf.
 
-Definition on_udecl_prop (Σ : global_env) (udecl : universes_decl)
-  := let levels := levels_of_udecl udecl in
-     let global_levels := global_levels Σ.(universes) in
-     let all_levels := LevelSet.union levels global_levels in
-     ConstraintSet.For_all (declared_cstr_levels all_levels) (constraints_of_udecl udecl).
-     (* /\ match udecl with
-       | Monomorphic_ctx ctx => LevelSet.for_all (negb ∘ Level.is_var) ctx.1
-                               /\ LevelSet.Subset ctx.1 global_levels
-                               /\ ConstraintSet.Subset ctx.2 (global_constraints Σ)
-                               /\ satisfiable_udecl Σ.(universes) udecl
-       | _ => True
-       end. *)
-
-Lemma in_global_levels l u : 
-  LevelSet.In l (ContextSet.levels u) ->
-  LevelSet.In l (global_levels u).
-Proof.
-  intros hin; now apply LevelSet.union_spec.
-Qed.
-
-Lemma weaken_lookup_on_global_env' Σ c decl :
-  wf Σ ->
-  lookup_env Σ c = Some decl ->
-  on_udecl_prop Σ (universes_decl_of_decl decl).
-Proof.
-  intros [onu wfΣ] HH.
-  destruct Σ as [univs Σ]; cbn in *.
-  induction wfΣ; simpl. 1: discriminate.
-  cbn in HH. subst udecl.
-  destruct (eqb_spec c kn); subst.
-  - apply some_inj in HH; destruct HH. subst.
-    clear -o. unfold on_udecl, on_udecl_prop in *.
-    destruct o as [H1 [H2 [H3 H4]]]. repeat split.
-    clear -H2. intros [[? ?] ?] Hc. specialize (H2 _ Hc).
-    destruct H2 as [H H']. simpl. split.
-    * apply LevelSet.union_spec in H. apply LevelSet.union_spec.
-      destruct H; [now left|right]; auto.
-    * apply LevelSet.union_spec in H'. apply LevelSet.union_spec.
-      destruct H'; [now left|right]; auto.
-    (*+ revert H3. case_eq (universes_decl_of_decl d); trivial.
-      intros ctx eq Hctx. repeat split.
-      * auto.
-      * intros l Hl. simpl. replace (monomorphic_levels_decl d) with ctx.1.
-        -- apply in_global_levels. apply LevelSet.union_spec; now left.
-        -- clear -eq. destruct d as [c|c]; cbn in *.
-           all: destruct c; cbn in *; now rewrite eq.
-      * simpl. replace (monomorphic_constraints_decl d) with ctx.2.
-        -- intros c Hc; apply ConstraintSet.union_spec; now left.
-        -- clear -eq. destruct d as [c|c]; cbn in *.
-           all: destruct c; cbn in *; now rewrite eq.
-      * clear -eq H4. destruct H4 as [v Hv]. exists v.
-      intros c Hc; apply (Hv c).
-      apply ConstraintSet.union_spec in Hc; destruct Hc as [Hc|Hc].
-      2: apply ConstraintSet.union_spec in Hc; destruct Hc as [Hc|Hc].
-      -- apply ConstraintSet.union_spec. simpl in *. left; now rewrite eq.
-      -- apply ConstraintSet.union_spec; left. simpl.
-         destruct d as [[? ? []]|[? ? ? ? []]]; simpl in *; tas;
-           now apply ConstraintSet.empty_spec in Hc.
-      -- apply ConstraintSet.union_spec; now right.*)
-  - specialize (IHwfΣ HH). revert IHwfΣ o; clear.
-    generalize (universes_decl_of_decl decl); intros d' HH Hd.
-    unfold on_udecl_prop in *.
-    intros [[? ?] ?] Hc. specialize (HH _ Hc).
-    destruct HH as [H' H'']. simpl. split.
-    * apply LevelSet.union_spec in H'. apply LevelSet.union_spec.
-      destruct H'; [now left|right]; auto.
-    * apply LevelSet.union_spec in H''. apply LevelSet.union_spec.
-      destruct H''; [now left|right]; auto.
-      
-    (*+ destruct d'; trivial. repeat split.
-      * destruct H2; auto.
-      * intros l Hl. apply H2 in Hl.
-        apply LevelSet.union_spec; now right.
-      * intros c Hc. apply H2 in Hc.
-        apply ConstraintSet.union_spec; now right.
-      * destruct Hd as [_ [_ [_ Hd]]]; cbn in Hd.
-        destruct Hd as [v Hv]. exists v. intros c Hc; apply Hv; clear v Hv.
-          apply ConstraintSet.union_spec in Hc; destruct Hc as [Hc|Hc]; simpl in *.
-          2: apply ConstraintSet.union_spec in Hc; destruct Hc as [Hc|Hc];
-            simpl in *.
-          -- apply H2 in Hc. apply ConstraintSet.union_spec; now right.
-          -- clear -Hc. destruct d as [[? ? []]|[? ? ? ? []]]; cbn in *.
-             all: try (apply ConstraintSet.empty_spec in Hc; contradiction).
-             all: apply ConstraintSet.union_spec; now left.
-          -- apply ConstraintSet.union_spec; now right.*)
-Qed.
-
-Lemma declared_cstr_levels_sub l l' c : 
-  LevelSet.Subset l l' ->
-  declared_cstr_levels l c -> declared_cstr_levels l' c.
-Proof.
-  intros sub; unfold declared_cstr_levels.
-  destruct c as [[l1 eq] l2]. intuition auto.
-Qed.
-
-Lemma on_udecl_on_udecl_prop (Σ : global_env) ctx :
-  on_udecl Σ.(universes) (Polymorphic_ctx ctx) -> on_udecl_prop Σ (Polymorphic_ctx ctx).
-Proof.
-  intros [? [? ?]]. red.
-  intros x hin. specialize (H0 x hin).
-  eapply declared_cstr_levels_sub; tea.
-  intros x' hin'.
-  eapply LevelSet.union_spec. apply LevelSet.union_spec in hin'.
-  intuition auto.
-Qed.
-
-Definition weaken_env_prop
-           (P : global_env_ext -> context -> term -> typ_or_sort -> Type) :=
-  forall Σ Σ' φ, wf Σ -> wf Σ' -> extends Σ Σ' -> forall Γ t T, P (Σ, φ) Γ t T -> P (Σ', φ) Γ t T.
-
-Definition weaken_env_decls_prop
-  (P : global_env_ext -> context -> term -> typ_or_sort -> Type) :=
-  forall Σ Σ' φ, wf Σ' -> extends_decls Σ Σ' -> forall Γ t T, P (Σ, φ) Γ t T -> P (Σ', φ) Γ t T.
-
-Lemma extends_decls_wf Σ Σ' : 
-  wf Σ' -> extends_decls Σ Σ' -> wf Σ.
-Proof.
-  intros [onu ond] [eq [Σ'' eq']].
-  split => //. 
-  - red. rewrite eq. apply onu.
-  - rewrite eq. rewrite eq' in ond.
-    revert ond; clear.
-    induction Σ''; cbn; auto.
-    intros H; depelim H.
-    apply IHΣ''. apply H.
-Qed. 
-
-End Extends.
-
-#[global] Hint Resolve extends_lookup : extends.
-#[global] Hint Resolve weakening_env_declared_constant : extends.
-#[global] Hint Resolve weakening_env_declared_minductive : extends.
-#[global] Hint Resolve weakening_env_declared_inductive : extends.
-#[global] Hint Resolve weakening_env_declared_constructor : extends.
-#[global] Hint Resolve weakening_env_declared_projection : extends.
-#[global] Hint Resolve weakening_env_is_allowed_elimination : extends.
-#[global] Hint Resolve weakening_env_global_ext_levels : extends.
-#[global] Hint Resolve weakening_env_consistent_instance : extends.
+#[global] Hint Resolve weakening_env_conv_ctx : extends.
+#[global] Hint Resolve weakening_env_cumul_ctx : extends.
