pcuic/theories/Bidirectional/BDToPCUIC.v
@@ -1,7 +1,7 @@
 From Coq Require Import Bool List Arith Lia.
 From MetaCoq.Template Require Import config utils monad_utils.
 From MetaCoq.PCUIC Require Import PCUICAst PCUICAstUtils PCUICInduction PCUICLiftSubst PCUICTyping PCUICInversion PCUICInductives PCUICInductiveInversion PCUICEquality PCUICUnivSubst PCUICClosed PCUICSubstitution PCUICValidity PCUICCumulativity PCUICInductives PCUICWfUniverses PCUICContexts PCUICSpine PCUICSR PCUICWellScopedCumulativity PCUICConversion PCUICOnFreeVars PCUICWeakeningTyp PCUICUnivSubstitutionTyp PCUICClosedTyp PCUICUnivSubstitutionConv.
-From MetaCoq.PCUIC Require Import BDEnvironmentTyping BDTyping.
+From MetaCoq.PCUIC Require Import BDTyping.
 
 Require Import ssreflect ssrbool.
 From Equations Require Import Equations.
